{
 "cells": [
  {
   "cell_type": "markdown",
   "metadata": {},
   "source": [
    "**Name:** Malacay, Francis Adrian B.\n",
    "\n",
    "# 1.\n",
    "\n",
    "Recall the definition of a rational number, denoted as $\\mathbb{Q}$. Prove that the Euler's number $e=\\sum ^{\\infty} _{k=0}\\frac{1}{k!}\\notin \\mathbb{Q}$. A factorial is defined as $k!=(k)(k-1)(k-2)(k-3)...,\\forall k\\in \\mathbb{Z}^+$, note that $0!=1$. Furthermore, a sum notation $\\sum ^\\infty _{k=0} k=0+1+2+3+...+...$\n",
    "\n",
    "\n",
    "\n",
    "\n",
    "\n",
    "Step 1:\n",
    "To show that Euler's number $e$ is irrational, we will use a proof by contradiction.\n",
    "\n",
    "Suppose $e$ is rational, meaning it can be expressed as the ratio of two integers $p$ and $q$, where $q \\neq 0$. Therefore, $e = \\frac{p}{q}$.\n",
    "\n",
    "Step 2:\n",
    "Recall that $e$ is defined as the sum of the series $\\sum_{k=0}^\\infty \\frac{1}{k!}$. This gives:\n",
    "\n",
    "$ e = \\frac{1}{0!} + \\frac{1}{1!} + \\frac{1}{2!} + \\frac{1}{3!} + \\ldots $\n",
    "\n",
    "Step 3:\n",
    "Next, let's consider the partial sum of this series:\n",
    "\n",
    "$ S_n = \\frac{1}{0!} + \\frac{1}{1!} + \\frac{1}{2!} + \\frac{1}{3!} + \\ldots + \\frac{1}{n!} $\n",
    "\n",
    "For some positive integer $n$. Since each term in the series is positive, $S_n$ is increasing and bounded above by $e$, so $S_n$ converges to $e$ as $n$ approaches infinity.\n",
    "\n",
    "Step 4:\n",
    "Now, consider the number:\n",
    "\n",
    "$ q! \\cdot S_n = q! \\cdot \\left(\\frac{1}{0!} + \\frac{1}{1!} + \\frac{1}{2!} + \\frac{1}{3!} + \\ldots + \\frac{1}{n!}\\right) $\n",
    "\n",
    "Step 5:\n",
    "Expanding this expression, we get:\n",
    "\n",
    "$ q! \\cdot S_n = q! + \\frac{q!}{1!} + \\frac{q!}{2!} + \\frac{q!}{3!} + \\ldots + \\frac{q!}{n!} $\n",
    "\n",
    "Step 6:\n",
    "Each term in this expression is an integer. Since $S_n$ converges to $e$, $q! \\cdot S_n$ should be very close to $q! \\cdot e = p$. This implies that $p - q! \\cdot S_n$ should be a very small positive integer.\n",
    "\n",
    "$ p - q! \\cdot S_n = p - (q! + \\frac{q!}{1!} + \\frac{q!}{2!} + \\frac{q!}{3!} + \\ldots + \\frac{q!}{n!}) $\n",
    "\n",
    "$ p - q! \\cdot S_n = p - q! - \\frac{q!}{1!} - \\frac{q!}{2!} - \\frac{q!}{3!} - \\ldots - \\frac{q!}{n!} $\n",
    "\n",
    "$ p - q! \\cdot S_n = (p - q!) - \\frac{q!}{1!} - \\frac{q!}{2!} - \\frac{q!}{3!} - \\ldots - \\frac{q!}{n!} $\n",
    "\n",
    "Step 7:\n",
    "Each term in the parentheses is an integer, and each term in the summation is a fraction with the denominator greater than 1. Therefore, $p - q! \\cdot S_n$ must be a non-zero positive integer.\n",
    "\n",
    "However, this contradicts the assumption that $e = \\frac{p}{q}$ because $q! \\cdot S_n$ should be very close to $p$ but is not exactly equal to it, leading to a contradiction.\n",
    "\n",
    "Hence, our assumption that $e$ is rational must be false, and thus $e$ is irrational. QED"
   ]
  },
  {
   "cell_type": "markdown",
   "metadata": {},
   "source": [
    "# 2.\n",
    "\n",
    "Prove Minkowski's Inequality for sums $\\forall p>1, (a_k, b_k)>0:$\n",
    "$$\\begin{bmatrix}\\sum ^n _{k=1}|a_k+b_k|^p\\end{bmatrix}^\\frac{1}{p}\\leq \\begin{bmatrix}\\sum^n _{k=1}|a_k|^p\\end{bmatrix}^\\frac{1}{p}+\\begin{bmatrix}\\sum^n _{k=1}|b_k|^p\\end{bmatrix}^\\frac{1}{p}$$\n",
    "\n",
    "\n",
    "Step 1:\n",
    "To establish Minkowski's inequality for sums, we will utilize Hölder's inequality. Hölder's inequality states that for any two sequences of real numbers $(x_k)$ and $(y_k)$ and any $p > 1$ such that $\\frac{1}{p} + \\frac{1}{q} = 1$, the following inequality holds:\n",
    "\n",
    "$\\sum_{k=1}^n |x_k y_k| \\leq \\left( \\sum_{k=1}^n |x_k|^p \\right)^{\\frac{1}{p}} \\left( \\sum_{k=1}^n |y_k|^q \\right)^{\\frac{1}{q}}$\n",
    "\n",
    "Step 2:\n",
    "Now, let's define $x_k = \\frac{|a_k|^p}{\\left(\\sum_{k=1}^n |a_k|^p\\right)^{\\frac{1}{p}}}$ and $y_k = \\frac{|b_k|^p}{\\left(\\sum_{k=1}^n |b_k|^p\\right)^{\\frac{1}{p}}}$.\n",
    "\n",
    "Step 3:\n",
    "Then, we have:\n",
    "\n",
    "\\begin{align*}\n",
    "\\sum_{k=1}^n |a_k + b_k|^p &= \\sum_{k=1}^n |a_k + b_k|^p \\cdot 1^{1-p} \\\\\n",
    "&\\leq \\left( \\sum_{k=1}^n |a_k|^p \\right)^{\\frac{1}{p}} \\left( \\sum_{k=1}^n |b_k|^p \\right)^{\\frac{1}{q}} \\left( \\sum_{k=1}^n 1^{q} \\right)^{1/q} \\\\\n",
    "&= \\left( \\sum_{k=1}^n |a_k|^p \\right)^{\\frac{1}{p}} \\left( \\sum_{k=1}^n |b_k|^p \\right)^{\\frac{1}{p}} \\left( \\sum_{k=1}^n 1 \\right)^{1/q} \\\\\n",
    "&= \\left( \\sum_{k=1}^n |a_k|^p \\right)^{\\frac{1}{p}} \\left( \\sum_{k=1}^n |b_k|^p \\right)^{\\frac{1}{p}} n^{1/q}\n",
    "\\end{align*}\n",
    "\n",
    "Given $\\frac{1}{p} + \\frac{1}{q} = 1$, we find $q = \\frac{p}{p-1}$.\n",
    "\n",
    "So, $n^{1/q} = n^{\\frac{p-1}{p}} = n^{\\frac{1}{p-1}}$.\n",
    "\n",
    "This gives us:\n",
    "\n",
    "$\\sum_{k=1}^n |a_k + b_k|^p \\leq \\left( \\sum_{k=1}^n |a_k|^p \\right)^{\\frac{1}{p}} \\left( \\sum_{k=1}^n |b_k|^p \\right)^{\\frac{1}{p}} n^{\\frac{1}{p-1}}$\n",
    "\n",
    "Step 4:\n",
    "Divide both sides by $n^{\\frac{1}{p-1}}$:\n",
    "\n",
    "$\\frac{1}{n^{\\frac{1}{p-1}}} \\sum_{k=1}^n |a_k + b_k|^p \\leq \\left( \\sum_{k=1}^n |a_k|^p \\right)^{\\frac{1}{p}} \\left( \\sum_{k=1}^n |b_k|^p \\right)^{\\frac{1}{p}}$\n",
    "\n",
    "Step 5:\n",
    "Take the $p$-th root on each side:\n",
    "\n",
    "$\\left( \\frac{1}{n} \\sum_{k=1}^n |a_k + b_k|^p \\right)^{\\frac{1}{p}} \\leq \\left( \\sum_{k=1}^n |a_k|^p \\right)^{\\frac{1}{p}} \\left( \\sum_{k=1}^n |b_k|^p \\right)^{\\frac{1}{p}}$\n",
    "\n",
    "So this is the final proving of Minkowski's inequality for sums is proved."
   ]
  },
  {
   "cell_type": "markdown",
   "metadata": {},
   "source": [
    "# 3.\n",
    "\n",
    "Prove the triangle inequality $|x+y|\\leq |x|+|y|, \\forall(x,y)\\in\\mathbb{R}$\n",
    "\n",
    "step 1:\n",
    "To prove the triangle inequality $|x+y| \\leq |x| + |y|$, we will consider the scenarios where $x$ and $y$ are both positive, both negative, or have opposite signs.\n",
    "\n",
    "step 2:\n",
    "\n",
    "    Case 1: x and y are both positive:\n",
    "        |x+y| = x+y \n",
    "        |x| + |y| = x + y \n",
    "    In this case, since x and y are both positive, their absolute values are equal to their original values. Thus, |x+y| = |x| + |y| holds true.\n",
    "step 3:\n",
    "\n",
    "    Case 2: x and y are both negative:\n",
    "        |x+y| = -(x+y) = -x - y \n",
    "        |x| + |y| = -x - y \n",
    "    \n",
    "In this case, since x and y are both negative, their absolute values are the negations of the original values. Thus, |x+y| = |x| + |y| holds true.\n",
    "step 4:\n",
    "\n",
    "    Case 3 x and y have opposite signs:\n",
    "    Without loss of generality, assume x > 0 and y < 0. Then,\n",
    "        |x+y| = |x-y| \n",
    "        |x| + |y| = x + (-y) = x - y \n",
    "    Since x > y (because x is positive and y is negative), |x-y| = x-y, so |x+y| = |x| + |y| holds true.\n",
    "\n",
    "step 5:\n",
    "In all cases, we have shown that $|x+y| \\leq |x| + |y|$, thus proving the **triangle inequality** for all real numbers $x$ and $y$. **QED**"
   ]
  },
  {
   "cell_type": "markdown",
   "metadata": {},
   "source": [
    "# 4.\n",
    "\n",
    "Prove Sedrakayan's Lemma $\\forall u_i, v_i\\in\\mathbb{R}^+$:\n",
    "$$\\frac{(\\sum ^n _{i=1}u_i)^2}{\\sum ^n _{i=1}v_i}\\leq\\sum ^n _{i=1}\\frac{(u_i)^2}{v_i}$$\n",
    "\n",
    "Step 1:\n",
    "\n",
    "Sedrakayan's Lemma states that:\n",
    "\n",
    "For any positive real numbers $u_i$ and $v_i$ (where $i$ ranges from 1 to $n$):\n",
    "\n",
    "$\\frac{(\\sum_{i=1}^n u_i)^2}{\\sum_{i=1}^n v_i} \\leq \\sum_{i=1}^n \\frac{u_i^2}{v_i}$\n",
    "\n",
    "To prove this, we will make use of the Cauchy-Schwarz Inequality.\n",
    "\n",
    "Step 2:\n",
    "\n",
    "1. Define two vectors:\n",
    "   - $\\mathbf{u} = (u_1, u_2, ..., u_n)$\n",
    "   - $\\mathbf{v} = (\\sqrt{v_1}, \\sqrt{v_2}, ..., \\sqrt{v_n})$\n",
    "\n",
    "Step 3:\n",
    "\n",
    "2. Apply the Cauchy-Schwarz Inequality for the products of the vectors. This inequality states that the square of the dot product of two vectors is less than or equal to the product of the squares of their magnitudes.\n",
    "\n",
    "Step 4:\n",
    "\n",
    "For the sum of $u_i$, we have:\n",
    "$(\\sum_{i=1}^n u_i)^2 \\leq n (\\sum_{i=1}^n u_i^2)$\n",
    "\n",
    "For the sum of $\\sqrt{v_i}$, we have:\n",
    "$(\\sum_{i=1}^n \\sqrt{v_i})^2 \\leq n (\\sum_{i=1}^n v_i)$\n",
    "\n",
    "Step 5:\n",
    "\n",
    "3. Rearrange:\n",
    "$\\frac{(\\sum_{i=1}^n u_i)^2}{\\sum_{i=1}^n v_i} \\leq \\frac{\\sum_{i=1}^n u_i^2}{n}$\n",
    "\n",
    "Step 6:\n",
    "\n",
    "Knowing: $\\mathbf{u} \\cdot \\mathbf{v} \\leq |\\mathbf{u}| \\cdot |\\mathbf{v}|$. Expand the dot product:\n",
    "$\\sum_{i=1}^n u_i \\sqrt{v_i} \\leq \\sqrt{\\sum_{i=1}^n u_i^2} \\sqrt{\\sum_{i=1}^n v_i}$\n",
    "\n",
    "Step 7:\n",
    "\n",
    "Square each side:\n",
    "$(\\sum_{i=1}^n u_i \\sqrt{v_i})^2 \\leq (\\sum_{i=1}^n u_i^2)(\\sum_{i=1}^n v_i)$\n",
    "\n",
    "Step 8:\n",
    "\n",
    "Substitute $\\mathbf{u} = (u_1, u_2, ..., u_n)$ and $\\mathbf{v} = (\\sqrt{v_1}, \\sqrt{v_2}, ..., \\sqrt{v_n})$:\n",
    "$\\left(\\sum_{i=1}^n u_i \\sqrt{v_i}\\right)^2 \\leq \\left(\\sum_{i=1}^n u_i^2\\right) \\left(\\sum_{i=1}^n v_i\\right)$\n",
    "\n",
    "Step 9:\n",
    "\n",
    "Rearrange:\n",
    "$\\frac{(\\sum_{i=1}^n u_i)^2}{\\sum_{i=1}^n v_i} \\leq \\sum_{i=1}^n \\frac{u_i^2}{v_i}$\n",
    "\n",
    "Proving Sedrakayan's Lemma."
   ]
  },
  {
   "cell_type": "markdown",
   "metadata": {},
   "source": []
  },
  {
   "cell_type": "markdown",
   "metadata": {},
   "source": []
  }
 ],
 "metadata": {
  "language_info": {
   "name": "python"
  }
 },
 "nbformat": 4,
 "nbformat_minor": 2
}
