{
 "cells": [
  {
   "cell_type": "markdown",
   "metadata": {},
   "source": [
    "**Name:** Malacay, Francis Adrian B.\n"
   ]
  },
  {
   "cell_type": "markdown",
   "metadata": {},
   "source": [
    "\n",
    "\n",
    "Intructions:\n",
    "- Use Latex to write your solution.\n",
    "- Push your solution to your github repository.\n",
    "\n",
    "Task 1:\n",
    "Consider the following experiment:\n",
    "\n",
    "1. The experiment consists of $n$ identical trials.\n",
    "2. The outcome of each trial falls into one of $k$ classes or cells.\n",
    "3. The probability that the outcome of a single trial falls into cell $i$, is $p_i,i = 1,2,...,k$ and remains the same from trial to trial. Notice that $p_1+p_2+p_3+¬∑¬∑¬∑+p_k =1.$\n",
    "4. The trials are independent.\n",
    "5. The random variables of interest are $Y_1 , Y_2 , . . . , Y_k$, where $Y_i$ equals the number of trials for which the outcome falls into cell $i$. Notice that $Y_1 +Y_2 +Y_3 +¬∑¬∑¬∑+Y_k =n$.\n",
    "6. The joint probability distribution $P(y) = \\frac{n!}{y_1!y_2!y_3!...y_n!} P_1^{y_1} P_2^{y_2} P_3^{y_3}....P_n^{y_n}$\n",
    "\n",
    "Question 1: Show that the expected value $E[y] = \\Sigma y \\cdotp P(y) = n \\cdot p_i$\n",
    "\n",
    "step 1:\n",
    "The expected value of a random variable $Y_i$ is given by $E[Y_i] = \\sum_{y} y \\cdot P(y)$.\n",
    "\n",
    "step 2:\n",
    "Using the provided joint probability distribution, we can find $E[Y_i]$ as follows:\n",
    "\n",
    "$ E[Y_i] = \\sum_{y} y \\cdot P(y) = \\sum_{y} y \\cdot \\frac{n!}{y_1!y_2!y_3!\\cdots y_n!} P_1^{y_1} P_2^{y_2} P_3^{y_3}\\cdots P_n^{y_n} $\n",
    "\n",
    "step 3:\n",
    "Now, since $Y_i$ represents the number of trials where the outcome falls into cell $i$, \n",
    "\n",
    "step 4:\n",
    "we can observe that $Y_i$ will be equal to $n \\cdot p_i$, where $p_i$ is the probability of the outcome falling into cell $i$ in a single trial. \n",
    "\n",
    "step 5:\n",
    "Thus, $E[Y_i] = n \\cdot p_i$. QED\n",
    "\n",
    "Question 2: Given the following data\n",
    "\\begin{gather}\n",
    "\\begin{bmatrix}\n",
    "\\begin{array}{c|c}\n",
    "Age & Proportion \\\\\n",
    "18-24 & 0.18 \\\\\n",
    "25-34 & 0.23 \\\\\n",
    "35-44 & 0.16 \\\\\n",
    "45-64 & 0.27 \\\\\n",
    "65-100 & 0.16 \\\\\n",
    "\\end{array}\n",
    "\\end{bmatrix}\n",
    "\\end{gather}\n",
    "\n",
    "If 500 adults are sampled  randomly, find the probability rhat the sample contains 100 person between 18 and 24, 200 between, 200 between the ages of 25 and 34, and 200 between the ages of 45 and 64.. What is the expected value for to obtain a person in the 65 and above?\n",
    "\n",
    "step 1:\n",
    "We'll use the multinomial distribution formula to determine the likelihood that the sample will include a specific number of people in each age group:\n",
    "\n",
    "$ P(y_1, y_2, y_3, y_4, y_5) = \\frac{500!}{100! \\cdot 200! \\cdot 200! \\cdot 0! \\cdot 0!} \\times 0.18^{100} \\times 0.23^{200} \\times 0.16^{200} \\times 0.27^0 \\times 0.16^0 $\n",
    "\n",
    "step 2:\n",
    "Where:\n",
    "- $y_1 = 100$ (persons aged 18-24)\n",
    "- $y_2 = 200$ (persons aged 25-34)\n",
    "- $y_3 = 200$ (persons aged 35-44)\n",
    "- $y_4 = 0$ (persons aged 45-64)\n",
    "- $y_5 = 0$ (persons aged 65-100)\n",
    "\n",
    "Once the probability of each age group has been determined, we can compute the expected value to acquire an individual 65 years of age or older by multiplying the likelihood of each age group by the total number of individuals in that age group.\n",
    "\n",
    "step 3:\n",
    "Let $ p_{\\text{65+}} $ represent the probability that an individual is 65 years of age or older. \n",
    "\n",
    "step 4:\n",
    "We can get $ p_{\\text{65+}} $ by deducting the total of the probability of the other age groups from 1 since we already know the probabilities of all the other age groups:\n",
    "\n",
    "$ p_{\\text{65+}} = 1 - (0.18 + 0.23 + 0.16 + 0.27) = 0.16 $\n",
    "\n",
    "step 5:\n",
    "Using a sample of 500 individuals, we now multiply the probability $ p_{\\text{65+}} $ by the sample size to determine the predicted number of adults 65 and older:\n",
    "\n",
    "$ \\text{Expected number of persons aged 65 and above} = 500 \\times 0.16 = 80 $\n",
    "\n",
    "step 6:\n",
    "As a result, 80 is the predicted value for an individual in the sample who is 65 years of age or older."
   ]
  },
  {
   "cell_type": "markdown",
   "metadata": {
    "vscode": {
     "languageId": "plaintext"
    }
   },
   "source": [
    "Task 2: Consider the following experiment:\n",
    "\n",
    "1. The experiment consists of a fixed number, $n$, of identical trials.\n",
    "2. Each trial results in one of two outcomes: success, $S$, or failure, $F$.\n",
    "3. The probability of success on a single trial is equal to some value $p$ and remains the same from trial to trial. The probability of a failure is equal to q = $(1 ‚àí p)$.\n",
    "4. The trials are independent.\n",
    "5. The random variable of interest is $Y$ , the number of successes observed during the $n$ trials.\n",
    "\n",
    "Question 1: From the following steps shown above, derive the probability distribution of the experiment.\n",
    "\n",
    "Question 2: Show that the expectation of this probability distribution is $E[y] = \\Sigma y \\cdotp P(y) = np$.\n",
    "\n",
    "Question 3: Experience has shown that 30% of all persons afflicted by a certain illness recover. A drug company has developed a new medication. Ten people with the illness were selected at random and received the medication; nine recovered shortly thereafter. Suppose that the medication was absolutely worthless. What is the probability that at least nine of ten receiving the medication will recover?\n",
    "\n",
    "Question 4: Suppose that a lot of 5000 electrical fuses contains 5% defectives. If a sample of 5 fuses is tested, find the probability of observing at least one defective.\n",
    "\n",
    "\n",
    "Question 1: \n",
    "\n",
    "Step 1:\n",
    "Denote $Y=y$ where $y$ is success that is observed out of $n$ trials.\n",
    "\n",
    "Step 2:\n",
    "We can determine the probability of observing $ùë¶$ successes and $(ùëõ‚àíùë¶)$ failures using the binomial probability formula.\n",
    "$$ P(Y = y) = \\binom{n}{y} \\times p^y \\times (1 - p)^{n - y} $$\n",
    "\n",
    "Where:\n",
    "- $n$ is the fixed number of trials,\n",
    "- $p$ is the probability of success on a single trial,\n",
    "- $\\binom{n}{y}$ represents the number of ways to choose $y$ successes out of $n$ trials (combinations), and\n",
    "- $(1 - p)^{n - y}$ represents the probability of $(n - y)$ failures.\n",
    "\n",
    "Question 2:\n",
    "\n",
    "Step 1:\n",
    "$E[y]$ signifies the mean value of the random variable across multiple experiments, . It's computed by adding up the product of each outcome $y$ and its corresponding probability $P(y)$.\n",
    "\n",
    "Step 2:\n",
    "This time, $Y$ denotes the number of successes seen throughout $n$ trials, where $p$ is the probability of success in each trial. The probability distribution of $Y$ follows a binomial distribution.\n",
    "\n",
    "The probability mass function of a binomial distribution:\n",
    "$$ P(y) = \\binom{n}{y} p^y (1 - p)^{n - y} $$\n",
    "\n",
    "where $\\binom{n}{y}$ is the binomial coefficient.\n",
    "\n",
    "Step 3:\n",
    "Sum all given values of $y$ multiplied by their probabilities to find the expectation of $E[y]$:\n",
    "$$ E[y] = \\sum_{y=0}^{n} y \\cdot P(y) $$\n",
    "\n",
    "Step 4:\n",
    "Substitute the probability mass functio of the binomial distribution:\n",
    "$$ E[y] = \\sum_{y=0}^{n} y \\cdot \\binom{n}{y} p^y (1 - p)^{n - y} $$\n",
    "\n",
    "Step 5:\n",
    "Simplify the expression using the properties of the binomial coefficient and linearity of expectation:\n",
    "$$ E[y] = \\sum_{y=1}^{n} y \\cdot \\binom{n}{y} p^y (1 - p)^{n - y} $$\n",
    "\n",
    "$$ = \\sum_{y=1}^{n} \\frac{n!}{(y-1)!(n-y)!} p^y (1 - p)^{n - y} $$\n",
    "\n",
    "$$ = \\sum_{y=1}^{n} np \\sum_{y=1}^{n} \\binom{n-1}{y-1} p^{y-1} (1 - p)^{(n-1) - (y-1)} $$\n",
    "\n",
    "$$ = np \\sum_{k=0}^{n-1} \\binom{n-1}{k} p^k (1 - p)^{(n-1) - k} $$\n",
    "\n",
    "$$ = np \\cdot 1 $$\n",
    "\n",
    "$$ = np $$\n",
    "\n",
    "Question 3:\n",
    "\n",
    "Step 1: Binomial Mass Property Function\n",
    "\n",
    "$$ P(Y = 9) = \\binom{10}{9} \\times (0.30)^9 \\times (0.70)^1 $$\n",
    "$$ P(Y = 9) = 10 \\times (0.30)^9 \\times (0.70)^1 $$\n",
    "\n",
    "$$ P(Y = 9) \\approx 0.000137781 $$\n",
    "\n",
    "$$ P(Y = 10) = \\binom{10}{10} \\times (0.30)^{10} \\times (0.70)^0 $$\n",
    "\n",
    "$$ P(Y = 10) = (0.30)^{10} \\times 1 $$\n",
    "\n",
    "$$ P(Y = 10) \\approx 0.0000059049 $$\n",
    "\n",
    "Step 2: Add the results\n",
    "$$ P(Y \\geq 9) = P(Y = 9) + P(Y = 10) $$\n",
    "\n",
    "$$ P(Y \\geq 9) \\approx 0.000137781 + 0.0000059049 $$\n",
    "\n",
    "$$ P(Y \\geq 9) \\approx 0.0001436869 $$\n",
    "\n",
    "Given this, there is a 0.0001436869 or 0.014% chance that at least 9 out of 10 patients getting treatment would recover.\n",
    "\n",
    "Question 4:\n",
    "\n",
    "Given:\n",
    "\n",
    "- Number of trials, $n = 5$ (sampling 5 fuses)\n",
    "- Probability of success (defective fuse), $p = 0.05$\n",
    "- Probability of failure (non-defective fuse), $q = 1 - p = 1 - 0.05 = 0.95$\n",
    "\n",
    "Step 1: Using Binomial probability mass function\n",
    "$$ P(Y \\geq 1) = 1 - P(Y = 0) $$\n",
    "\n",
    "$$ = 1 - \\binom{5}{0} \\times 0.05^0 \\times 0.95^5 $$\n",
    "\n",
    "$$ = 1 - 1 \\times 1 \\times (0.95)^5 $$\n",
    "\n",
    "$$ = 1 - 1 \\times 1 \\times 0.7737809375$$\n",
    "\n",
    "$$ \\approx 1 - 0.7737809375 $$\n",
    "\n",
    "$$ \\approx 0.2262190625 $$\n",
    "\n",
    "The likelihood of finding at least one faulty fuse in a sample of five tested fuses is $0.2262$, or $22.62\\%$."
   ]
  },
  {
   "cell_type": "markdown",
   "metadata": {},
   "source": [
    "Task 3: Consider a probility distribution of $p(y) = \\frac{\\lambda^y}{y!} e^{-\\lambda}$.\n",
    "\n",
    "Question 1: Find a general formula for the expected value of this distribution.\n",
    "\n",
    "\n",
    "Step 1:\n",
    "Using the concept of the expected value for discrete random variables, we can get the expected value of the given probability distribution, which is a Poisson distribution with parameter $\\lambda$, represented as $E(Y)$:\n",
    "\n",
    "$$\n",
    "E(Y) = \\sum_{y=0}^{\\infty} y \\cdot p(y)\n",
    "$$\n",
    "\n",
    "Step 2:\n",
    "Substituting the expression for $p(y)$ given in the problem, we get:\n",
    "\n",
    "$$\n",
    "E(Y) = \\sum_{y=0}^{\\infty} y \\cdot \\frac{\\lambda^y}{y!} e^{-\\lambda}\n",
    "$$\n",
    "\n",
    "Step 3:\n",
    "We'll utilize the knowledge that a probability distribution's total probability is equal to $1$ to solve this. As a result, the total may be rewritten as follows:\n",
    "\n",
    "$$\n",
    "E(Y) = \\sum_{y=1}^{\\infty} y \\cdot \\frac{\\lambda^y}{y!} e^{-\\lambda} + 0 \\cdot \\frac{\\lambda^0}{0!} e^{-\\lambda}\n",
    "$$\n",
    "\n",
    "Step 4:\n",
    "Now, we can simplify the terms with $y$ greater than $0$:\n",
    "\n",
    "$$\n",
    "E(Y) = \\sum_{y=1}^{\\infty} y \\cdot \\frac{\\lambda^y}{y!} e^{-\\lambda}\n",
    "$$\n",
    "\n",
    "Step 5:\n",
    "To simplify further, let's take $e^{-\\lambda}$ outside the sum:\n",
    "\n",
    "$$\n",
    "E(Y) = e^{-\\lambda} \\sum_{y=1}^{\\infty} \\frac{\\lambda^y}{(y-1)!}\n",
    "$$\n",
    "\n",
    "Step 6:\n",
    "Let's now substitute anything to make the expression inside the sum simpler. Assuming $k = y - 1$, $y = k + 1$. Moreover, observe that $k = 0$ when $y = 1$, and that $k$ approaches infinity as well as $y$ approaches infinity. After making these changes, the total becomes:\n",
    "\n",
    "$$\n",
    "E(Y) = e^{-\\lambda} \\sum_{k=0}^{\\infty} \\frac{\\lambda^{k+1}}{k!}\n",
    "$$\n",
    "\n",
    "$$\n",
    "E(Y) = e^{-\\lambda} \\lambda \\sum_{k=0}^{\\infty} \\frac{\\lambda^k}{k!}\n",
    "$$\n",
    "\n",
    "Step 7:\n",
    "The sum inside the expression is recognizable as the Taylor series expansion of $e^\\lambda$, which is $e^\\lambda$. Therefore:\n",
    "\n",
    "$$\n",
    "E(Y) = e^{-\\lambda} \\lambda e^\\lambda\n",
    "$$\n",
    "\n",
    "$$\n",
    "E(Y) = \\lambda\n",
    "$$\n",
    "\n",
    "Step 8:\n",
    "Thus, $\\lambda$ is the universal formula for the expected value of the given distribution.\n",
    "\n",
    "Question 2: A certain type of tree has seedlings randomly dispersed in a large area, with the mean density of seedlings being approximately five per square yard. If a forester randomly locates ten 1-square-yard sampling regions in the area, find the probability that none of the regions will contain seedlings.\n",
    "\n",
    "\n",
    "Question 2:\n",
    "\n",
    "Given:\n",
    "$\\lambda = 5$\n",
    "<br>\n",
    "Step 1: Use Poisson distribution:\n",
    "$$P(Y = y) = \\frac{\\lambda^y}{y!} e^{-\\lambda}$$\n",
    "\n",
    "$$y = 0$$\n",
    "\n",
    "$$ P(Y = 0) = \\frac{5^0}{0!} e^{-5} $$\n",
    "\n",
    "$$ = e^{-5} $$\n",
    "Step 2: Calculate the probability\n",
    "\n",
    "$$P(Y = 0) \\approx e^{-5} $$\n",
    "\n",
    "$$\\approx 0.006737947$$\n",
    "\n",
    "There is a <b>.67%</b> chance that no areas will have any seedlings."
   ]
  }
 ],
 "metadata": {
  "language_info": {
   "name": "python"
  }
 },
 "nbformat": 4,
 "nbformat_minor": 2
}
